SSA/Projects/MLIRSyntax/EDSL.lean
@@ -411,14 +411,14 @@ macro_rules
 | `([mlir_type| tensor1d ]) => do
     `(MLIRType.tensor1d)
 
-def tensor1dTest : MLIRType := [mlir_type| tensor1d]
+def tensor1dTest : MLIRTy := [mlir_type| tensor1d]
 
 syntax "tensor2d" : mlir_type
 macro_rules
 | `([mlir_type| tensor2d ]) => do
     `(MLIRType.tensor2d)
 
-def tensor2dTest : MLIRType:= [mlir_type| tensor2d]
+def tensor2dTest : MLIRTy := [mlir_type| tensor2d]
 
 -- EDSL MLIR USER ATTRIBUTES
 -- =========================
@@ -451,7 +451,7 @@ syntax "[mlir_ops|" mlir_ops "]" : term
 
 macro_rules
 | `([mlir_ops| $[ $ops ]*  ]) => do
-      let initList: TSyntax `term <- `(@List.nil (MLIR.AST.Op))
+      let initList: TSyntax `term <- `(@List.nil (MLIR.AST.Op _))
       let l ← ops.foldrM (init := initList)
         fun x (xs: TSyntax `term) => `([mlir_op|$x] :: $xs)
       return l
@@ -466,7 +466,7 @@ syntax "[mlir_region|" mlir_region "]": term
 
 macro_rules
 | `([mlir_region| { ^ $name:ident ( $operands,* ) : $ops }  ]) => do
-   let initList <- `(@List.nil (MLIR.AST.SSAVal × MLIR.AST.MLIRType))
+   let initList <- `(@List.nil (MLIR.AST.SSAVal × MLIR.AST.MLIRType _))
    let argsList <- operands.getElems.foldrM (init := initList) fun x xs => `([mlir_bb_operand| $x] :: $xs)
    let opsList <- `([mlir_ops| $ops])
    `(Region.mk $(Lean.quote (name.getId.toString)) $argsList $opsList)
@@ -570,25 +570,25 @@ def attrVal0Str : AttrVal := [mlir_attr_val| "foo"]
 #reduce attrVal0Str
 
 -- Uses dialect coercion: empty → builtin
-example : AttrValue := [mlir_attr_val| "foo"]
+example : AttrVal := [mlir_attr_val| "foo"]
 -- Uses dialect coercion: empty → empty + builtin
 --example : AttrValue (Dialect.empty + builtin) := [mlir_attr_val| "foo"]
 -- Uses dialect coercion after building an AttrValue Dialect.empty
 
 
-def attrVal1bTy : AttrValue := [mlir_attr_val| i32]
+def attrVal1bTy : AttrVal := [mlir_attr_val| i32]
 #reduce attrVal1bTy
 
-def attrVal2List : AttrValue := [mlir_attr_val| ["foo", "foo"] ]
+def attrVal2List : AttrVal := [mlir_attr_val| ["foo", "foo"] ]
 #reduce attrVal2List
 
-def attrVal3AffineMap : AttrValue := [mlir_attr_val| affine_map<(x, y) -> (y)>]
+def attrVal3AffineMap : AttrVal := [mlir_attr_val| affine_map<(x, y) -> (y)>]
 #reduce attrVal3AffineMap
 
-def attrVal4Symbol : AttrValue := [mlir_attr_val| @"foo" ]
+def attrVal4Symbol : AttrVal := [mlir_attr_val| @"foo" ]
 #reduce attrVal4Symbol
 
-def attrVal5int: AttrValue := [mlir_attr_val| 42 ]
+def attrVal5int: AttrVal := [mlir_attr_val| 42 ]
 #reduce attrVal5int
 
 def attrVal5bint: AttrVal := [mlir_attr_val| -42 ]
@@ -660,7 +660,7 @@ macro_rules
 
 
 
-def attr0Str : AttrEntry := [mlir_attr_entry| sym_name = "add"]
+def attr0Str : AttrEntry 0 := [mlir_attr_entry| sym_name = "add"]
 #print attr0Str
 
 -- def attr2Escape : AttrEntry builtin :=
@@ -669,11 +669,11 @@ def attr0Str : AttrEntry := [mlir_attr_entry| sym_name = "add"]
 -- #print attr0Str
 
 
-def attr3Unit : AttrEntry :=
+def attr3Unit : AttrEntry 0 :=
    [mlir_attr_entry| sym_name]
 #print attr3Unit
 
-def attr4Negative : AttrEntry :=
+def attr4Negative : AttrEntry 0 :=
    [mlir_attr_entry| value = -1: i32]
 #reduce attr4Negative
 
@@ -685,12 +685,12 @@ syntax "[mlir_attr_dict|" mlir_attr_dict "]" : term
 macro_rules
 | `([mlir_attr_dict| {  $attrEntries,* } ]) => do
         let attrsList <- attrEntries.getElems.toList.mapM (fun x => `([mlir_attr_entry| $x]))
-        let attrsList <- quoteMList attrsList (<- `(MLIR.AST.AttrEntry))
+        let attrsList <- quoteMList attrsList (<- `(MLIR.AST.AttrEntry _))
         `(AttrDict.mk $attrsList)
 
-def attrDict0 : AttrDict := [mlir_attr_dict| {}]
-def attrDict1 : AttrDict := [mlir_attr_dict| {foo = "bar" }]
-def attrDict2 : AttrDict := [mlir_attr_dict| {foo = "bar", baz = "quux" }]
+def attrDict0 : AttrDict 0 := [mlir_attr_dict| {}]
+def attrDict1 : AttrDict 0 := [mlir_attr_dict| {foo = "bar" }]
+def attrDict2 : AttrDict 0 := [mlir_attr_dict| {foo = "bar", baz = "quux" }]
 
 -- dict attribute val
 syntax mlir_attr_dict : mlir_attr_val
@@ -698,7 +698,7 @@ syntax mlir_attr_dict : mlir_attr_val
 macro_rules
 | `([mlir_attr_val| $v:mlir_attr_dict]) => `(AttrValue.dict [mlir_attr_dict| $v])
 
-def nestedAttrDict0 : AttrDict := [mlir_attr_dict| {foo = {bar = "baz"} }]
+def nestedAttrDict0 : AttrDict 0 := [mlir_attr_dict| {foo = {bar = "baz"} }]
 #print nestedAttrDict0
 
 -- MLIR OPS WITH REGIONS AND ATTRIBUTES AND BASIC BLOCK ARGS
@@ -729,7 +729,7 @@ macro_rules
 
         -- TODO: Needs a consistency check that `resName=none ↔ resType=.unit`
         let res ← match resName with
-        | none => `(@List.nil (MLIR.AST.TypedSSAVal))
+        | none => `(@List.nil (MLIR.AST.TypedSSAVal _))
         | some name =>
            match resTypes.getElems with
            | #[] => Macro.throwError s!"expected to have return type since result '{resName}' exists"
@@ -741,15 +741,15 @@ macro_rules
         let operands: List (MacroM <| TSyntax `term) :=
           List.zipWith (fun x y => `(([mlir_op_operand| $x], [mlir_type| $y])))
           operandsNames.getElems.toList operandsTypes.getElems.toList
-        let operands ← quoteMList (← operands.mapM id) (← `(MLIR.AST.TypedSSAVal))
+        let operands ← quoteMList (← operands.mapM id) (← `(MLIR.AST.TypedSSAVal _))
         let attrDict <- match attrDict with
                           | none => `(AttrDict.mk [])
                           | some dict => `([mlir_attr_dict| $dict])
         let rgnsList <- match rgns with
-                  | none => `(@List.nil (MLIR.AST.Region))
+                  | none => `(@List.nil (MLIR.AST.Region _))
                   | some rgns => do
                     let rngs <- rgns.getElems.mapM (fun x => `([mlir_region| $x]))
-                    quoteMList rngs.toList (<- `(MLIR.AST.Region))
+                    quoteMList rngs.toList (<- `(MLIR.AST.Region _))
 
         `(Op.mk $name -- name
                 $res -- results
@@ -765,47 +765,36 @@ syntax mlir_op_operand "="
 
 macro_rules
   | `([mlir_op|
-        $resName:mlir_op_operand =
-        $name:str
-        ( $operandsNames,* )
-        $[ ( $rgns,* ) ]?
-        $[ $attrDict ]?
-        : ( $operandsTypes,* ) -> $resType:mlir_type  ]) => do
-
-        let res ←   `([([mlir_op_operand| $resName], [mlir_type| $resType])])
+        $resName:mlir_op_operand = $name:str ( $operandsNames,* ) $[ ( $rgns,* ) ]? $[ $attrDict ]?
+        : ( $operandsTypes,* ) -> $resType:mlir_type  
+      ]) => do
+        let results ← `([([mlir_op_operand| $resName], [mlir_type| $resType])])
         -- TODO: Needs a consistency check that `operandsNames.length = operandsTypes.length`
         let operands: List (MacroM <| TSyntax `term) :=
           List.zipWith (fun x y => `(([mlir_op_operand| $x], [mlir_type| $y])))
           operandsNames.getElems.toList operandsTypes.getElems.toList
-        let operands ← quoteMList (← operands.mapM id) (← `(MLIR.AST.TypedSSAVal))
-        let attrDict <- match attrDict with
+        let operands ← quoteMList (← operands.mapM id) (← `(MLIR.AST.TypedSSAVal _))
+        let attributes <- match attrDict with
                           | none => `(AttrDict.mk [])
                           | some dict => `([mlir_attr_dict| $dict])
-        let rgnsList <- match rgns with
-                  | none => `(@List.nil (MLIR.AST.Region))
+        let regions <- match rgns with
+                  | none => `(@List.nil (MLIR.AST.Region _))
                   | some rgns => do
                     let rngs <- rgns.getElems.mapM (fun x => `([mlir_region| $x]))
-                    quoteMList rngs.toList (<- `(MLIR.AST.Region))
+                    quoteMList rngs.toList (<- `(MLIR.AST.Region _))
+        `(Op.mk $name $results $operands $regions $attributes)
 
-        `(Op.mk $name -- name
-                $res -- results
-                $operands -- operands
-                $rgnsList -- regions
-                $attrDict) -- attrs
-
-
-
-def op1 : Op :=
+def op1 : Op φ :=
   [mlir_op| "foo"(%x, %y) : (i32, i32) -> (i32) ]
 #print op1
-def op2: Op :=
+def op2: Op φ :=
   [mlir_op| %z = "foo"(%x, %y) : (i32, i32) -> (i32)]
 #print op2
 
-def bbop1 : SSAVal × MLIRTy := [mlir_bb_operand| %x : i32 ]
+def bbop1 : SSAVal × MLIRTy φ := [mlir_bb_operand| %x : i32 ]
 #print bbop1
 
-def bb1NoArgs : Region :=
+def bb1NoArgs : Region φ :=
   [mlir_region| {
      ^entry:
      "foo"(%x, %y) : (i32, i32) -> (i32)
@@ -814,7 +803,7 @@ def bb1NoArgs : Region :=
   }]
 #print bb1NoArgs
 
-def bb2SingleArg : Region :=
+def bb2SingleArg : Region φ :=
   [mlir_region| {
      ^entry(%argp : i32):
      "foo"(%x, %y) : (i32, i32) -> (i32)
@@ -824,7 +813,7 @@ def bb2SingleArg : Region :=
 #print bb2SingleArg
 
 
-def bb3MultipleArgs : Region :=
+def bb3MultipleArgs : Region φ :=
   [mlir_region| {
      ^entry(%argp : i32, %argq : i64):
      "foo"(%x, %y) : (i32, i32) -> (i32)
@@ -834,17 +823,17 @@ def bb3MultipleArgs : Region :=
 #reduce bb3MultipleArgs
 
 
-def rgn0 : Region  := ([mlir_region|  { }])
+def rgn0 : Region φ := ([mlir_region|  { }])
 #print rgn0
 
-def rgn1 : Region :=
+def rgn1 : Region φ :=
   [mlir_region|  {
     ^entry:
       "std.return"(%x0) : (i42) -> ()
   }]
 #print rgn1
 
-def rgn2 : Region :=
+def rgn2 : Region φ :=
   [mlir_region|  {
     ^entry:
       "std.return"(%x0) : (i42) -> ()
@@ -852,7 +841,7 @@ def rgn2 : Region :=
 #print rgn2
 
 -- | test what happens if we try to use an entry block with no explicit bb name
-def rgn3 : Region :=
+def rgn3 : Region φ :=
   [mlir_region|  {
       "std.return"(%x0) : (i42) -> ()
   }]
@@ -860,18 +849,18 @@ def rgn3 : Region :=
 
 
 -- | test simple ops [no regions]
-def opcall1 : Op := [mlir_op| "foo" (%x, %y) : (i32, i32) -> (i32) ]
+def opcall1 : Op φ := [mlir_op| "foo" (%x, %y) : (i32, i32) -> (i32) ]
 #print opcall1
 
 
 
-def oprgn0 : Op := [mlir_op|
+def oprgn0 : Op φ := [mlir_op|
  "func"() ({ ^entry: %x = "foo.add"() : () -> (i64) } ) : () -> ()
 ]
 #reduce oprgn0
 
 -- | note that this is a "full stack" example!
-def opRgnAttr0 : Op := [mlir_op|
+def opRgnAttr0 : Op φ := [mlir_op|
  "module"() ({
   ^entry:
    "func"() ({
@@ -900,7 +889,7 @@ macro_rules
 | `([mlir_op| func $name:mlir_attr_val_symbol ( $args,* ) $[ -> $ret:mlir_type ]? { $ops } ]) => do
      -- Make the arguments for the entry block
      let bbargs ← args.getElems.mapM (fun x => `([mlir_bb_operand| $x]))
-     let bbargs ← quoteMList bbargs.toList (← `(MLIR.AST.SSAVal × MLIR.AST.MLIRType))
+     let bbargs ← quoteMList bbargs.toList (← `(MLIR.AST.SSAVal × MLIR.AST.MLIRType _))
      -- Make the entry block (the only block)
      let rgn ← `(Region.mk "entry" $bbargs [mlir_ops| $ops])
 
@@ -930,10 +919,10 @@ macro_rules
      let rgn <- `(Region.fromOps $ops)
      `(Op.mk "module" [] [] [$rgn] AttrDict.empty)
 
-def mod1 : Op := [mlir_op| module { }]
+def mod1 : Op φ := [mlir_op| module { }]
 #print mod1
 
-def mod2 : Op := [mlir_op| module { "dummy.dummy"(): () -> () }]
+def mod2 : Op φ := [mlir_op| module { "dummy.dummy"(): () -> () }]
 #print mod2
 
 end MLIR.EDSL
